finished monotonicity for interval analysis

spa.v
@@ -27,29 +27,6 @@ Definition join (a1 a2 : alv) : alv :=
         else top
     end
   end.
-
-Theorem join_commutative : forall a b : alv, join a b = join b a.
-Proof.
-  intros. destruct a; destruct b; try reflexivity. simpl.
-  replace (base =? base0) with (base0 =? base).
-  replace (ptr =? ptr0) with (ptr0 =? ptr).
-  replace (bound =? bound0) with (bound0 =? bound).
-  destruct ((base0 =? base) && (ptr0 =? ptr) && (bound0 =? bound)) eqn:B.
-  - destruct (base0 =? base) eqn:B1;
-    destruct (ptr0 =? ptr) eqn:B2;
-    destruct (bound0 =? bound) eqn:B3; try discriminate.
-    + apply Nat.eqb_eq in B1.
-      apply Nat.eqb_eq in B2.
-      apply Nat.eqb_eq in B3.
-      rewrite B1. rewrite B2. rewrite B3.
-      replace (max size size0) with (max size0 size).
-      { reflexivity. }
-      { apply Nat.max_comm. }
-  - reflexivity.
-  - apply eqb_sym.
-  - apply eqb_sym.
-  - apply eqb_sym.
-Qed.
   
 Hint Constructors leq : core.
 
@@ -88,71 +65,39 @@ Proof.
      destruct ((base =? ba) && (ptr =? p) && (bound =? bo)) eqn:B; auto.
      apply ofst_leq_ofst. lia.
 Qed.
-  
-
-(*
-(** Assume the following CFG:
-
-            A   B
-             \ /
-              C
-              
-  Then, if [[A]](v) = X and [[B]](v) = Y, we need to "merge" X and Y into the least upper bound of the two,
-  in order to conduct a conservative analysis, which will then be used as the input to block C. 
-  This is what the following join function does.
-*) 
-Inductive join : alv -> alv -> alv -> Prop :=
-  | join_bot_bot :                                    join Bottom Bottom Bottom
-  | join_bot_ofst :       forall n : nat,             join Bottom (FPOffset n) (FPOffset n)
-  | join_bot_top :                                    join Bottom Top Top
-  | join_ofst_bot :       forall n : nat,             join (FPOffset n) Bottom (FPOffset n)
-  | join_ofst_ofst_eq :   forall n m : nat, n = m ->  join (FPOffset n) (FPOffset m) (FPOffset m)
-  | join_ofst_ofst_neq :  forall n m : nat, n <> m -> join (FPOffset n) (FPOffset m) Top
-  | join_ofst_top :       forall n : nat,             join (FPOffset n) Top Top
-  | join_top_bot :                                    join Top Bottom Top
-  | join_top_ofst :       forall n : nat,             join Top (FPOffset n) Top
-  | join_top_top :                                    join Top Top Top.
 
 
-Hint Constructors leq : core.
-
-Theorem join_func_is_monotonic : forall x y z a b: alv, 
-    (leq x y -> join x z a /\ join y z b -> leq a b)
- /\ (leq y z -> join x y a /\ join x z b -> leq a b).
-Proof.
-  intros. split; intros L J; destruct J as [J1 J2].
-    - inversion L; destruct z; subst; inversion J1; inversion J2; subst; auto.  
-    - inversion L; destruct x; subst; inversion J1; inversion J2; subst; auto. 
-Qed.
-
-(** For the purposes of stack points-to analysis, we need only care about instructions that may produce pointers. Each such instruction falls into one of the following categories. *)
 Inductive llvm_instruction : Type :=
-  | static_alloca (base_fp_offset : nat)                    (* static alloca insns always have an offset from frame pointer *)
-  | bitcast (a : alv)                                       (* the ALV here refers to the ALV mapped to the bitcast's operand variable *)
-  | get_element_pointer (base : alv) (base_offset : alv)    (* the ALVs here refer to those mapped to the base and offset variables for the GEP instruction *)
-  | other.                                                  (* represents every other instruction that assigns a variable *)
+  | static_alloca (typ_size fp_ofst : nat)
+  | bitcast (typ_size : nat)
+  | gep (typ_size : nat) (ofst : nat)
+  | other.
   
-(** For each of the pointer-producing instructions, the following propositions specify how the variable being assigned gets its abstract lattice value.
-
-  We can read a proposition of the form `flow_rule insn a b` as: 
-    " after performing instruction `v = insn`, the initial mapping v-->a will now be v-->b " 
- *)
-Inductive flow_rule : llvm_instruction -> alv -> alv -> Prop :=
-  | alloca_rule :             forall (prev : alv) (ofst : nat),               flow_rule (static_alloca ofst) prev (FPOffset ofst)
-  | bitcast_rule :            forall (prev bc_operand : alv)   ,              flow_rule (bitcast bc_operand) prev bc_operand
-  | gep_rule_both_eq_ofst  :  forall (prev : alv) (base_ofst buf_ofst : nat), 
-                                                                              flow_rule (get_element_pointer (FPOffset base_ofst) (FPOffset buf_ofst)) prev (FPOffset (base_ofst + buf_ofst))
-  | gep_rule_one_neq_ofst :   forall (prev base_operand buf_operand : alv) (base_ofst buf_ofst : nat), 
-                                base_operand <> FPOffset(base_ofst) \/ buf_operand <> FPOffset(buf_ofst) 
-                                                                          ->  flow_rule (get_element_pointer base_operand buf_operand) prev Top                                                                  
-  | other_rule :              forall (prev : alv),                            flow_rule (other) prev (Top).
-
-
-Theorem flow_rules_are_monotonic : forall (x y z a b : alv) (insn : llvm_instruction),
-    leq x y -> flow_rule insn x a /\ flow_rule insn x b -> leq a b.
+  
+Definition flow_rule (insn : llvm_instruction) (operand_alv : alv) : alv :=
+  match insn with
+  | static_alloca (typ_size) (fp_ofst) => 
+      fpoffset fp_ofst fp_ofst (fp_ofst + typ_size) typ_size
+  | bitcast (typ_size) =>
+      match operand_alv with
+      | top => top
+      | bottom => bottom
+      | fpoffset base ptr bound size =>
+          fpoffset base ptr bound typ_size
+      end
+  | gep (typ_size) (ofst) => 
+      match operand_alv with
+      | top => top
+      | bottom => bottom
+      | fpoffset base ptr bound size =>
+          fpoffset base (ptr + ofst) bound typ_size
+      end
+  | other => top
+  end.
+  
+Theorem flow_rules_monotonic : forall insn op1 op2, 
+  leq op1 op2 -> leq (flow_rule insn op1) (flow_rule insn op2).
 Proof.
-  intros x y z a b insn L [F1 F2]. destruct insn;
-  try (inversion L; inversion F1; inversion F2; subst; auto); 
-  destruct b; auto.
-Qed.     *)
-
+  intros insn op1 op2 L.
+  destruct insn; inversion L; subst; simpl; auto.
+Qed.
